examples/riscv/isqrt/isqrt_symb_transfScript.sml
@@ -66,4 +66,157 @@ Proof
  rw [bir_isqrt_prog_def,bspec_cont_2_thm]
 QED
 
+(* branch contract *)
+
+val init_addr_tm = (snd o dest_eq o concl) isqrt_init_addr_3_def;
+val end_addr_1_tm = (snd o dest_eq o concl) isqrt_end_addr_3_loop_def;
+val end_addr_2_tm = (snd o dest_eq o concl) isqrt_end_addr_3_ret_def;
+
+val bspec_pre_tm = (lhs o snd o strip_forall o concl) bspec_isqrt_pre_3_def;
+val bspec_post_1_tm = (lhs o snd o strip_forall o concl) bspec_isqrt_post_3_loop_def;
+val bspec_post_2_tm = (lhs o snd o strip_forall o concl) bspec_isqrt_post_3_ret_def;
+
+val bir_prog_def = bir_isqrt_prog_def;
+val birenvtyl_def = isqrt_birenvtyl_def;
+val bspec_pre_def = bspec_isqrt_pre_3_def;
+val bspec_post_1_def = isqrt_end_addr_3_loop_def;
+val bspec_post_2_def = isqrt_end_addr_3_ret_def;
+val prog_vars_def = isqrt_prog_vars_def;
+val symb_analysis_thm = isqrt_symb_analysis_3_thm;
+val bsysprecond_thm = isqrt_bsysprecond_3_thm;
+val prog_vars_thm = isqrt_prog_vars_thm;
+
+(* ---- *)
+
+open birs_stepLib;
+open birs_composeLib;
+open birs_driveLib;
+open birs_auxTheory;
+
+open HolBACoreSimps;
+open bir_typing_expTheory;
+
+open pred_setTheory;
+open distribute_generic_stuffTheory;
+
+val birs_state_ss = rewrites (type_rws ``:birs_state_t``);
+val bprog_tm = (fst o dest_eq o concl) bir_prog_def;
+val prog_vars_tm = (fst o dest_eq o concl) prog_vars_def;
+val birenvtyl_tm = (fst o dest_eq o concl) birenvtyl_def;
+val bir_state_init_lbl_tm = (snd o dest_eq o concl o EVAL)
+ ``bir_block_pc (BL_Address (Imm64 ^init_addr_tm))``;
+
+val birs_state_end_lbl_1_tm = (snd o dest_eq o concl o EVAL)
+ ``bir_block_pc (BL_Address (Imm64 ^end_addr_1_tm))``;
+val birs_state_end_lbl_2_tm = (snd o dest_eq o concl o EVAL)
+ ``bir_block_pc (BL_Address (Imm64 ^end_addr_2_tm))``;
+
+val birs_state_init_pre_tm =
+``birs_state_init_pre_GEN ^bir_state_init_lbl_tm ^birenvtyl_tm
+  (mk_bsysprecond ^bspec_pre_tm ^birenvtyl_tm)``;
+
+val (sys_i, L_s, Pi_f) = (symb_sound_struct_get_sysLPi_fun o concl) symb_analysis_thm;
+
+Theorem analysis_L_INTER_EMPTY[local]:
+ {^birs_state_end_lbl_1_tm; ^birs_state_end_lbl_2_tm} INTER ^L_s = {}
+Proof
+ EVAL_TAC
+QED
+
+val birs_state_init_pre_EQ_thm =
+  prove (``^((snd o dest_comb) sys_i) = ^birs_state_init_pre_tm``,
+   REWRITE_TAC [birs_state_init_pre_GEN_def, mk_bsysprecond_def, bsysprecond_thm] >>
+   CONV_TAC (computeLib.RESTR_EVAL_CONV [``birs_eval_exp``] THENC birs_stepLib.birs_eval_exp_CONV));
+
+val analysis_thm =
+  REWRITE_RULE [birs_state_init_pre_EQ_thm, GSYM bir_prog_def] symb_analysis_thm;
+
+val birenvtyl_EVAL_thm =
+ (REWRITE_CONV [
+     birenvtyl_def,
+     bir_lifting_machinesTheory.riscv_bmr_vars_EVAL,
+     bir_lifting_machinesTheory.riscv_bmr_temp_vars_EVAL] THENC EVAL)
+   birenvtyl_tm;
+
+val birs_state_thm = REWRITE_CONV [birenvtyl_EVAL_thm] birs_state_init_pre_tm;
+
+val birs_symb_symbols_f_sound_prog_thm =
+  (SPEC (inst [Type`:'observation_type` |-> Type.alpha] bprog_tm)
+    bir_symb_soundTheory.birs_symb_symbols_f_sound_thm);
+
+val birs_prop_transfer_thm =
+  (MATCH_MP symb_prop_transferTheory.symb_prop_transfer_thm
+    birs_symb_symbols_f_sound_prog_thm);
+
+val type_of_bir_exp_thms =
+    let
+      open bir_immTheory
+      open bir_valuesTheory
+      open bir_envTheory
+      open bir_exp_memTheory
+      open bir_bool_expTheory
+      open bir_extra_expsTheory
+      open bir_nzcv_expTheory
+      open bir_interval_expTheory
+    in [
+      type_of_bir_exp_def,
+      bir_var_type_def,
+      bir_type_is_Imm_def,
+      type_of_bir_imm_def,
+      BExp_Aligned_type_of,
+      BExp_unchanged_mem_interval_distinct_type_of,
+      bir_number_of_mem_splits_REWRS,
+      BType_Bool_def,
+      bir_exp_true_def,
+      bir_exp_false_def,
+      BExp_MSB_type_of,
+      BExp_nzcv_ADD_DEFS,
+      BExp_nzcv_SUB_DEFS,
+      n2bs_def,
+      BExp_word_bit_def,
+      BExp_Align_type_of,
+      BExp_ror_type_of,
+      BExp_LSB_type_of,
+      BExp_word_bit_exp_type_of,
+      BExp_ADD_WITH_CARRY_type_of,
+      BExp_word_reverse_type_of,
+      BExp_ror_exp_type_of
+    ] end;
+
+val bprog_P_entails_thm =
+ prove (``P_entails_an_interpret
+  (bir_symb_rec_sbir ^bprog_tm)
+  (P_bircont ^birenvtyl_tm ^bspec_pre_tm)
+  (birs_symb_to_symbst ^birs_state_init_pre_tm)``,
+
+ ASSUME_TAC (GSYM prog_vars_thm) >>
+ `^prog_vars_tm = MAP PairToBVar ^birenvtyl_tm` by (
+  SIMP_TAC std_ss [birenvtyl_def, listTheory.MAP_MAP_o,
+   PairToBVar_BVarToPair_I_thm, listTheory.MAP_ID]) >>
+ POP_ASSUM (fn thm => FULL_SIMP_TAC std_ss [thm]) >>
+ IMP_RES_TAC (SIMP_RULE std_ss [] P_bircont_entails_thm) >>
+ SIMP_TAC std_ss [] >>
+ POP_ASSUM (ASSUME_TAC o SPEC bspec_pre_tm) >>
+ `bir_vars_of_exp ^bspec_pre_tm SUBSET set (MAP PairToBVar ^birenvtyl_tm)` by EVAL_TAC >>
+ POP_ASSUM (fn thm => FULL_SIMP_TAC std_ss [thm]) >>
+ `ALL_DISTINCT (MAP FST ^birenvtyl_tm)` by EVAL_TAC >>
+ POP_ASSUM (fn thm => FULL_SIMP_TAC std_ss [thm]) >>
+ `IS_SOME (type_of_bir_exp ^bspec_pre_tm)` by (
+   SIMP_TAC std_ss [bspec_pre_def] >>
+   CONV_TAC (RAND_CONV (SIMP_CONV (srw_ss()) type_of_bir_exp_thms)) >>
+   SIMP_TAC (std_ss++holBACore_ss) [optionTheory.option_CLAUSES]
+ ) >>
+ POP_ASSUM (fn thm => FULL_SIMP_TAC std_ss [thm]));
+
+val sys1 = (snd o dest_eq o concl o REWRITE_CONV [bsysprecond_thm]) birs_state_init_pre_tm;
+
+val (Pi_func, Pi_set) = dest_comb Pi_f;
+
+val sys2s = pred_setSyntax.strip_set Pi_set;
+
+val sys2s_posts = [];
+
+val label_0 = (snd o dest_eq o concl o EVAL) `` ^(List.nth (sys2s,0)).bsst_pc``;
+val label_1 = (snd o dest_eq o concl o EVAL) `` ^(List.nth (sys2s,1)).bsst_pc``;
+
 val _ = export_theory ();
